

# Snars 7

Michał Iwicki, Agata Osmałek

December 2, 2025

## P7.1

The master equation:

$$N_k(t+1) - N_k(t) = \frac{k-1}{2t} N_{k-1}(t) - \frac{k}{2t} N_k(t) + \delta_{k,m}, \quad (1)$$

where  $m$  is the minimum degree and number of links each new node brings.

The stationary distribution is defined as:

$$P(k) = \lim_{t \rightarrow \infty} \frac{N_k(t)}{t}. \quad (2)$$

For large  $t$ , we can approximate  $N_k(t+1) \approx N_k(t)$  and  $\frac{N_k(t)}{t} \approx P(k)$  to obtain:

$$0 = \frac{k-1}{2} P(k-1) - \frac{k}{2} P(k) + \delta_{k,m}. \quad (3)$$

For  $k > m$ , this yields a recurrence:

$$P(k) = \frac{k-1}{k+2} P(k-1). \quad (4)$$

To determine  $P(m)$ , use the  $k = m$  case:

$$P(m) = \frac{2}{m+2}. \quad (5)$$

Repeated application of the recurrence gives the closed form

$$P(k) = \frac{2m(m+1)}{k(k+1)(k+2)}. \quad (6)$$

As  $k \rightarrow \infty$ ,  $P(k) \sim k^{-3}$ , recovering the BA exponent  $\gamma = 3$ .

## P7.4

### Definition of $Q(k)$

The distribution  $Q(k)$  is defined as the probability that a node at the end of a randomly chosen edge has degree  $k$ . It therefore differs from  $P(k)$ , which is the degree distribution of a randomly selected vertex.

## Counting Argument

The number of vertices with degree  $k$  is approximately  $NP(k)$ . Each vertex of degree  $k$  contributes exactly  $k$  edge ends. Hence, the total number of edge ends connected to vertices of degree  $k$  equals

$$kNP(k).$$

The total number of all edge ends in the network is equal to the sum of all degrees:

$$N\langle k \rangle.$$

## Derivation of $Q(k)$

The probability that a randomly chosen edge end is attached to a vertex of degree  $k$  is given by

$$Q(k) = \frac{kNP(k)}{N\langle k \rangle}.$$

Canceling the factor  $N$ , we obtain

$$Q(k) = \frac{k}{\langle k \rangle} P(k).$$

## Interpretation

Vertices with a larger degree are more likely to be reached by following a randomly selected edge. This explains the additional factor  $k$  in the relation between  $Q(k)$  and  $P(k)$ .

## P7.5

When traversing a network by following randomly chosen edges, the degree distribution of the reached vertices is not given by  $P(k)$ , but by the excess degree distribution

$$Q(k) = \frac{kP(k)}{\langle k \rangle},$$

since vertices with higher degree are more likely to be reached.

If a vertex of degree  $k$  is reached by following an edge, one of its edges has already been used. Therefore, the number of *new* outgoing edges available for further spreading is  $k - 1$ . The average branching factor of the network is thus given by

$$B = \sum_k (k - 1)Q(k).$$

The percolation threshold corresponds to the critical point at which the branching process becomes self-sustaining, i.e.

$$B = 1.$$

This condition can be rewritten as

$$\sum_k (k-1)Q(k) = 1 \iff \sum_k kQ(k) = 2.$$

Using the definition of  $Q(k)$ , we obtain

$$\sum_k kQ(k) = \sum_k k \frac{kP(k)}{\langle k \rangle} = \frac{1}{\langle k \rangle} \sum_k k^2 P(k) = \frac{\langle k^2 \rangle}{\langle k \rangle}.$$

Thus, the condition for the existence of a giant connected component (or, equivalently, for percolation) is

$$\frac{\langle k^2 \rangle}{\langle k \rangle} \geq 2.$$

This criterion shows that the emergence of large-scale connectivity is governed by the ratio of the second to the first moment of the degree distribution.

## P7.6

### Degree Distribution in ER Graphs

For Erdős–Rényi graphs, the degree distribution follows a Poisson distribution with mean

$$\lambda = \langle k \rangle.$$

The first two moments are given by

$$\langle k \rangle = \lambda, \quad \langle k^2 \rangle = \lambda^2 + \lambda.$$

### Applying the Percolation Condition

Substituting these moments into the percolation criterion derived in Task 7.5 yields

$$\frac{\langle k^2 \rangle}{\langle k \rangle} = \frac{\lambda^2 + \lambda}{\lambda} = \lambda + 1.$$

### Critical Threshold

At the percolation threshold the equality holds:

$$\lambda + 1 = 2,$$

which implies

$$\lambda = 1.$$

Hence, the critical average degree is

$$\langle k \rangle_c = 1.$$

Since for ER graphs  $\langle k \rangle \approx pN$ , the critical connection probability is

$$p_c \approx \frac{1}{N}.$$

## P7.8

Let  $G_0(x) = \sum_{k=0}^{\infty} P(k)x^k$ .

**(a)**  $G_0(1) = 1$

This follows directly from normalization  $\sum_k P(k) = 1$  as  $x = 1$ .

**(b)**  $G'_0(1) = \langle k \rangle$

Differentiating, we obtain:

$$G'_0(x) = \sum_k kP(k)x^{k-1}, \quad (7)$$

then evaluating at  $x = 1$ :

$$G'_0(1) = \sum_k kP(k), \quad (8)$$

$P(k)$  can be seen as a fraction of all nodes that has a degree  $k$  meaning, that the sum corresponds to the average degree:

$$G'_0(1) = \langle k \rangle, \quad (9)$$

**(c)**  $\frac{d}{dx}[xG'_0(x)]\big|_{x=1} = \langle k^2 \rangle$

Calculate:

$$\begin{aligned} \frac{d}{dx}[xG'_0(x)] &= G'_0(x) + xG''_0(x), \\ G''_0(x) &= \sum_k k(k-1)P(k)x^{k-2} \end{aligned}$$

$$\frac{d}{dx}[xG'_0(x)]_{x=1} = \sum_k kP(k) + \sum_k k(k-1)P(k) = \sum_k kP(k)[1 + (k-1)] = \sum_k k^2P(k) = \langle k^2 \rangle.$$

**(d)**  $G_1(x) = \frac{G'_0(x)}{G'_0(1)}$

Let's recall:

$$F(k) = \frac{k+1}{\langle k \rangle} P(k+1). \quad (10)$$

Then:

$$G_1(x) = \sum_{k=0}^{\infty} F(k)x^k = \frac{1}{\langle k \rangle} \sum_{j=1}^{\infty} jP(j)x^{j-1} = \frac{G'_0(x)}{G'_0(1)}. \quad (11)$$

(e)  $G'_1(1) = \frac{\langle k^2 \rangle}{\langle k \rangle} - 1$

Differentiating  $G_1(x)$ :

$$G'_1(x) = \frac{G''_0(x)}{G'_0(1)} = \frac{\langle k^2 \rangle - \langle k \rangle}{\langle k \rangle}. \quad (12)$$

For  $x=1$ :

$$G'_1(1) = \frac{G''_0(1)}{G'_0(1)} = \frac{\sum_k k(k-1)P(k)}{\langle k \rangle} = \frac{\sum_k k^2 P(k) - \sum_k k P(k)}{\langle k \rangle} = \frac{\langle k^2 \rangle - \langle k \rangle}{\langle k \rangle}. \quad (13)$$

## P7.9

For a Poisson degree distribution:

$$P(k) = e^{-\langle k \rangle} \frac{\langle k \rangle^k}{k!}, \quad (14)$$

calculate:

$$G_0(x) = e^{-\langle k \rangle} \sum_{k=0}^{\infty} \frac{(\langle k \rangle x)^k}{k!} = e^{-\langle k \rangle} e^{\langle k \rangle x} = e^{\langle k \rangle (x-1)}. \quad (15)$$

## P7.10

Using  $G_1(x) = G'_0(x)/G'_0(1)$  and  $G_0(x) = e^{\langle k \rangle (x-1)}$ , we have:

$$G_1(x) = e^{\langle k \rangle (x-1)} = G_0(x). \quad (16)$$

## P7.11

$h_1(s)$  is the probability that starting from the end of a randomly selected edge, we can explore  $s$  vertices in finite number of steps.

Arriving at a vertex via an edge yields the excess-degree distribution  $F(k)$ , meaning the vertex has  $k$  additional edges. If these  $k$  branches collectively contribute  $s-1$  nodes (probability of which is described as  $h_k(s-1)$ ), then, to get a distribution over any randomly chosen edge, you need to sum over all values  $k = 0 \dots s-1$ , yielding:

$$h_1(s) = \sum_{k=0}^{s-1} F(k) h_k(s-1). \quad (17)$$

## P7.12

(a)  $H_1(x) = x \sum_{k=0} F(k) H_k(x)$

$$H_1(x) = \sum_{s=0}^{\infty} h_1(s) x^s = \sum_{s=0}^{\infty} \left[ \sum_{k=0}^{s-1} F(k) h_k(s-1) \right] x^s = x \sum_{s=1}^{\infty} \sum_{k=0}^{s-1} F(k) h_k(s-1) x^{s-1} =$$

$$= x \sum_k F(k) \sum_{s=1}^{\infty} h_k(s-1)x^{s-1} = x \sum_k F(k) \sum_{s=0}^{\infty} h_k(s)x^s = x \sum_k F(k)H_k(x)$$

**(b)**  $H_k(x) = [H_1(x)]^k$

If there are  $k$  independent branches, each one has distribution generated by  $H_1(x)$ . The sum of independent random variables corresponds to multiplication of generating functions. Thus, the distribution of sum of all the independent branches has a generating function of:

$$H_k(x) = [H_1(x)]^k$$

**(c)**  $H_1(x) = xG_1(H_1(x))$

Using P7.11:

$$H_1(x) = \sum_s x^s \sum_k F(k)h_k(s-1) = x \sum_k F(k)H_k(x) = x \sum_k F(k)[H_1(x)]^k = xG_1(H_1(x)). \quad (18)$$

**(d)**  $H_0(x) = xG_0(H_1(x))$

$$H_0(x) = \sum_s \sum_k P(k)h_k(s)x^s = x \sum_k P(k) \sum_s h_k(s)x^s = x \sum_k P(k)H_k(x) = x \sum_k P(k)[H_1(x)]^k = xG_0(H_1(x)) \quad (19)$$

## P7.13

$$\langle s \rangle = H'_0(1) = 1 + G'_0(1)H'_1(1). \quad (20)$$

Differentiate  $H_1(x) = xG_1(H_1(x))$ :

$$H'_1(x) = G_1(H_1(x)) + xG'_1(H_1(x))H'_1(x). \quad (21)$$

Set  $x = 1$ , use  $G_1(1) = 1$  and  $H_1(1) = 1$ :

$$H'_1(1) = 1 + G'_1(1)H'_1(1) \quad \Rightarrow \quad H'_1(1) = \frac{1}{1 - G'_1(1)}. \quad (22)$$

Use  $G'_1(1) = \frac{\langle k^2 \rangle}{\langle k \rangle} - 1$  to obtain

$$H'_1(1) = \frac{\langle k \rangle}{2\langle k \rangle - \langle k^2 \rangle}. \quad (23)$$

Thus

$$\langle s \rangle = 1 + \frac{\langle k \rangle^2}{2\langle k \rangle - \langle k^2 \rangle}. \quad (24)$$

## P7.14

Let  $v = H_1(1)$ . The fixed-point condition is

$$v = G_1(v). \quad (25)$$

The probability is

$$P_\infty = 1 - H_0(1) = 1 - G_0(v). \quad (26)$$

For ER, using  $G_0 = G_1 = e^{\langle k \rangle (x-1)}$ , we compute

$$v = e^{\langle k \rangle (v-1)}, \quad (27)$$

so with  $v = 1 - P_\infty$  we obtain the equation:

$$P_\infty = 1 - e^{-\langle k \rangle P_\infty}. \quad (28)$$

## P7.16

$$P(k) = (\alpha - 1)m^{\alpha-1}k^{-\alpha}, \quad k = m, \dots, k_{\max}, \quad (29)$$

with  $k_{\max} = mN^{1/(\alpha-1)}$ .

$$\begin{aligned} \langle k \rangle &= \int_m^{k_{\max}} k \frac{(\alpha - 1)m^{\alpha-1}}{k^\alpha} = \frac{\alpha - 1}{2 - \alpha} m^{\alpha-1} [k_{\max}^{2-\alpha} - m^{2-\alpha}] \\ \langle k^2 \rangle &= \int_m^{k_{\max}} k^2 \frac{(\alpha - 1)m^{\alpha-1}}{k^\alpha} = \frac{\alpha - 1}{3 - \alpha} m^{\alpha-1} [k_{\max}^{3-\alpha} - m^{3-\alpha}] \end{aligned}$$

Let's set  $C = (\alpha - 1)m^{\alpha-1}$  and consider cases:

- $3 < \alpha$  - elements  $(2 - \alpha)$ ,  $(3 - \alpha)$  are negative so those parts vanish when  $k_{\max} \rightarrow \infty$

$$\langle k \rangle = C \frac{-m^{2-\alpha}}{2 - \alpha} = \frac{1 - \alpha}{2 - \alpha} m$$

$$\langle k^2 \rangle = C \frac{-m^{3-\alpha}}{3 - \alpha} = \frac{1 - \alpha}{3 - \alpha} m^2$$

$$\frac{\langle k^2 \rangle}{\langle k \rangle} = \left| \frac{2 - \alpha}{3 - \alpha} \right| m$$

- $2 < \alpha < 3$  - then  $(2 - \alpha) < 0$ , but  $(3 - \alpha) > 0$ . When  $k_{\max} \rightarrow \infty$

$$\langle k \rangle = C \frac{-m^{2-\alpha}}{2 - \alpha} = \frac{1 - \alpha}{2 - \alpha} m$$

$$\langle k^2 \rangle = C \frac{k_{\max}^{3-\alpha} - m^{3-\alpha}}{3 - \alpha} = \frac{1 - \alpha}{3 - \alpha} (m^2 - m^{\alpha-1} k_{\max}^{3-\alpha})$$

$$\frac{\langle k^2 \rangle}{\langle k \rangle} = \frac{2 - \alpha}{3 - \alpha} (m - m^{\alpha-2} k_{\max}^{3-\alpha}) \approx \left| \frac{2 - \alpha}{3 - \alpha} \right| m^{\alpha-2} k_{\max}^{3-\alpha} \quad \text{for } k_{\max} \gg m$$

- $\alpha < 2$  - then both  $(2 - \alpha)$  and  $(3 - \alpha)$  are positive. When  $k_{max} \rightarrow \infty$

$$\langle k \rangle = C \frac{k_{max}^{2-\alpha} - m^{2-\alpha}}{2 - \alpha} = \frac{1 - \alpha}{2 - \alpha} (m - m^{\alpha-1} k_{max}^{2-\alpha}) \approx \frac{1 - \alpha}{2 - \alpha} (-m^{\alpha-1} k_{max}^{2-\alpha}) \quad \text{for } k_{max} \gg m$$

$$\langle k^2 \rangle = C \frac{k_{max}^{3-\alpha} - m^{3-\alpha}}{3 - \alpha} = \frac{1 - \alpha}{3 - \alpha} (m^2 - m^{\alpha-1} k_{max}^{3-\alpha}) \approx \frac{1 - \alpha}{3 - \alpha} (-m^{\alpha-1} k_{max}^{3-\alpha}) \quad \text{for } k_{max} \gg m$$

$$\frac{\langle k^2 \rangle}{\langle k \rangle} \approx \left| \frac{2 - \alpha}{3 - \alpha} \right| k_{max} \quad \text{for } k_{max} \gg m$$

## P7.17

Having degree distribution of scale-free network:

$$P(k) = (\alpha - 1) k_{min}^{\alpha-1} k^{-\alpha}$$

And the polylogarithm function:

$$Li_{\alpha}(x) = \sum_{k=1}^{\infty} \frac{x^k}{k^{\alpha}}$$

From definition of  $G_0$ :

$$G_0(x) = \sum_{k=0}^{\infty} P(k) x^k = \sum_{k=0}^{\infty} (\alpha - 1) k_{min}^{\alpha-1} k^{-\alpha} x^k = (\alpha - 1) k_{min}^{\alpha-1} \sum_{k=1}^{\infty} k^{-\alpha} x^k = (\alpha - 1) k_{min}^{\alpha-1} Li_{\alpha}(x)$$

For  $k_{min} = 1$ :

$$G_0(x) = (\alpha - 1) Li_{\alpha}(x)$$

Diffrentiating:

$$G'_0(x) = (\alpha - 1) \sum_{k=1}^{\infty} k \frac{x^{k-1}}{k^{\alpha}} = (\alpha - 1) \frac{1}{x} \sum_{k=1}^{\infty} \frac{x^k}{k^{\alpha-1}} = \frac{(\alpha - 1)}{x} Li_{\alpha-1}(x)$$

As for  $G_1$ :

$$G_1(x) = \frac{G'_0(x)}{G'_0(1)} = \frac{\frac{(\alpha-1)}{x} Li_{\alpha-1}(x)}{\langle k \rangle}$$

From P.16, for  $\alpha > 2$  we have:  $\frac{1-\alpha}{2-\alpha} k_{min}$  using this for  $k_{min} = 1$  we get:

$$G_1(x) = \frac{\frac{(\alpha-1)}{x} Li_{\alpha-1}(x)}{\frac{1-\alpha}{2-\alpha}} = \frac{\alpha - 2}{x} Li_{\alpha-1}(x)$$